converting MutableBtree to be datataype-in-class

examples/MutableBtree.dfy
@@ -24,61 +24,66 @@ abstract module MutableBtree {
   function method DefaultValue() : Value
   function method DefaultKey() : Key
 
-  datatype Node =
-    | NotInUse // For not-currently-in-use entries in children arrays
-    | Leaf(ghost repr: set<object>, ghost height: nat, nkeys: uint64, keys: array<Key>, values: array<Value>)
-    | Index(ghost repr: set<object>, ghost height: nat, nchildren: uint64, pivots: array<Key>, children: array<Node>)
+  class Node {
+    var contents: NodeContents
+    ghost var repr: set<object>
+    ghost var height: nat
+  }
+    
+  datatype NodeContents =
+    | Leaf(nkeys: uint64, keys: array<Key>, values: array<Value>)
+    | Index(nchildren: uint64, pivots: array<Key>, children: array<Node?>)
 
-  predicate DisjointSubtrees(node: Node, i: int, j: int)
+  predicate DisjointSubtrees(node: NodeContents, i: int, j: int)
     requires node.Index?
     requires 0 <= i < node.children.Length
     requires 0 <= j < node.children.Length
-    requires !node.children[i].NotInUse?
-    requires !node.children[j].NotInUse?
+    requires node.children[i] != null
+    requires node.children[j] != null
     requires i != j
-    reads node.children
+    reads node.children, node.children[i], node.children[j]
   {
     node.children[i].repr !! node.children[j].repr
   }
 
-  predicate {:fuel 2} WFShape(node: Node)
-    reads if node.NotInUse? then {} else node.repr
-    decreases if node.NotInUse? then {} else node.repr
+  predicate WFShape(node: Node)
+    reads node, node.repr
+    decreases node.height
   {
-    if node.NotInUse? then false
-    else if node.Leaf? then
-      && node.repr == { node.keys, node.values }
-      && node.keys != node.values
+    if node.contents.Leaf? then
+      && node.repr == { node.contents.keys, node.contents.values }
+      && node.contents.keys != node.contents.values
       && node.height == 0
-      && 0 <= node.nkeys as int <= MaxKeysPerLeaf() as int == node.keys.Length
-      && node.values.Length == node.keys.Length
-    else 
-      && node.pivots in node.repr
-      && node.children in node.repr
-      && 0 < node.nchildren as int <= MaxChildren() as int == node.children.Length
-      && node.pivots.Length == MaxChildren() as int - 1
-      && (forall i :: 0 <= i < node.nchildren ==> !node.children[i].NotInUse?)
-      && (forall i :: 0 <= i < node.nchildren ==> node.children[i].repr < node.repr)
-      && (forall i :: 0 <= i < node.nchildren as int ==> node.pivots !in node.children[i].repr)
-      && (forall i :: 0 <= i < node.nchildren as int ==> node.children !in node.children[i].repr)
-      && (forall i, j :: 0 <= i < j < node.nchildren as int ==> DisjointSubtrees(node, i, j))
-      && (forall i :: 0 <= i < node.nchildren ==> node.children[i].height < node.height)
-      && (forall i :: 0 <= i < node.nchildren ==> WFShape(node.children[i]))
+      && 0 <= node.contents.nkeys as int <= MaxKeysPerLeaf() as int == node.contents.keys.Length
+      && node.contents.values.Length == node.contents.keys.Length
+    else
+      && {node, node.contents.pivots, node.contents.children} <= node.repr
+      && 0 < node.contents.nchildren as int <= MaxChildren() as int == node.contents.children.Length
+      && node.contents.pivots.Length == MaxChildren() as int - 1
+      && (forall i :: 0 <= i < node.contents.nchildren ==> node.contents.children[i] != null)
+      && (forall i :: 0 <= i < node.contents.nchildren ==> node.contents.children[i] in node.repr)
+      && (forall i :: 0 <= i < node.contents.nchildren ==> node.contents.children[i].repr < node.repr)
+      && (forall i :: 0 <= i < node.contents.nchildren ==> node !in node.contents.children[i].repr)
+      && (forall i :: 0 <= i < node.contents.nchildren ==> node.contents.pivots !in node.contents.children[i].repr)
+      && (forall i :: 0 <= i < node.contents.nchildren ==> node.contents.children !in node.contents.children[i].repr)
+      && (forall i, j :: 0 <= i < j < node.contents.nchildren as int ==> DisjointSubtrees(node.contents, i, j))
+      && (forall i :: 0 <= i < node.contents.nchildren ==> node.contents.children[i].height < node.height)
+      && (forall i :: 0 <= i < node.contents.nchildren ==> WFShape(node.contents.children[i]))
   }
 
   predicate ObjectIsInSubtree(node: Node, o: object, i: int)
     requires WFShape(node)
-    requires node.Index?
-    requires 0 <= i < node.nchildren as int
+    requires node.contents.Index?
+    requires 0 <= i < node.contents.nchildren as int
     reads node.repr
   {
-    o in node.children[i].repr
+    o in node.contents.children[i].repr
   }
 
   function {:opaque} SubRepr(node: Node, from: int, to: int) : (result: set<object>)
     requires WFShape(node)
-    requires node.Index?
-    requires 0 <= from <= to <= node.nchildren as int
+    requires node.contents.Index?
+    requires 0 <= from <= to <= node.contents.nchildren as int
     reads node.repr
   {
     set i: int, o | 0 <= from <= i < to && o in node.repr && ObjectIsInSubtree(node, o, i) :: o
@@ -86,8 +91,8 @@ abstract module MutableBtree {
 
   lemma SubReprsDisjoint(node: Node, from1: int, to1: int, from2: int, to2: int)
     requires WFShape(node)
-    requires node.Index?
-    requires 0 <= from1 <= to1 <= from2 <= to2 <= node.nchildren as int
+    requires node.contents.Index?
+    requires 0 <= from1 <= to1 <= from2 <= to2 <= node.contents.nchildren as int
     ensures SubRepr(node, from1, to1) !! SubRepr(node, from2, to2)
   {
     var subrepr1 := SubRepr(node, from1, to1);
@@ -98,28 +103,29 @@ abstract module MutableBtree {
       var i1 :| 0 <= from1 <= i1 < to1 && o in node.repr && ObjectIsInSubtree(node, o, i1);
       var i2 :| 0 <= from2 <= i2 < to2 && o in node.repr && ObjectIsInSubtree(node, o, i2);
       assert i1 < i2;
-      assert DisjointSubtrees(node, i1, i2);
+      assert DisjointSubtrees(node.contents, i1, i2);
     }
   }
   
   lemma SubReprFits(node: Node, from: int, to: int)
     requires WFShape(node)
-    requires node.Index?
-    requires 1 < node.nchildren
-    requires 0 <= from <= to <= node.nchildren as int
-    ensures SubRepr(node, from, to) <= node.repr - {node.pivots, node.children}
-    ensures to - from < node.nchildren as int ==> SubRepr(node, from, to) < node.repr - {node.pivots, node.children}
-    ensures forall i :: from <= i < to ==> node.children[i].repr <= SubRepr(node, from, to)
+    requires node.contents.Index?
+    requires 1 < node.contents.nchildren
+    requires 0 <= from <= to <= node.contents.nchildren as int
+    ensures SubRepr(node, from, to) <= node.repr - {node, node.contents.pivots, node.contents.children}
+    ensures to - from < node.contents.nchildren as int ==> SubRepr(node, from, to) < node.repr - {node, node.contents.pivots, node.contents.children}
+    ensures forall i :: from <= i < to ==> node.contents.children[i].repr <= SubRepr(node, from, to)
   {
     var subrepr := SubRepr(node, from, to);
-    var nchildren := node.nchildren;
-    var children := node.children;
+    var nchildren := node.contents.nchildren;
+    var pivots := node.contents.pivots;
+    var children := node.contents.children;
     
     reveal_SubRepr();
     assert subrepr <= node.repr;
-    assert node.pivots !in subrepr;
-    assert node.children !in subrepr;
-    assert subrepr <= node.repr - {node.pivots, node.children};
+    assert pivots !in subrepr;
+    assert children !in subrepr;
+    assert subrepr <= node.repr - {node, pivots, children};
     
     if to - from < nchildren as int {
       assert children[0].repr < node.repr;
@@ -130,29 +136,29 @@ abstract module MutableBtree {
         forall o | o in subrepr
           ensures o !in children[0].repr
         {
-          if o == node.pivots {
+          if o == pivots {
           } else if o == children {
           } else {
             var i :| from <= i < to && o in node.repr && ObjectIsInSubtree(node, o, i);
-            assert DisjointSubtrees(node, 0, i);
+            assert DisjointSubtrees(node.contents, 0, i);
           }
         }
-        assert subrepr < node.repr - {node.pivots, node.children};
+        assert subrepr < node.repr - {node, pivots, children};
       } else {
         assert to < nchildren as int;
         forall o | o in subrepr
           ensures o !in children[nchildren - 1].repr
         {
-          if o == node.pivots {
+          if o == pivots {
           } else if o == children {
           } else {
             var i :| from <= i < to && o in node.repr && ObjectIsInSubtree(node, o, i);
-            assert DisjointSubtrees(node, i, nchildren as int - 1);
+            assert DisjointSubtrees(node.contents, i, nchildren as int - 1);
           }
         }
         var wit :| wit in children[nchildren-1].repr;
         assert wit !in subrepr;
-        assert subrepr < node.repr - {node.pivots, node.children};
+        assert subrepr < node.repr - {node, pivots, children};
       }
     }
     forall i | from <= i < to
@@ -166,762 +172,762 @@ abstract module MutableBtree {
     }
   }
   
-  function method IndexPrefix(node: Node, newnchildren: int) : (result: Node)
-    requires WFShape(node)
-    requires node.Index?
-    requires 1 < node.nchildren
-    requires 0 <= newnchildren <= node.nchildren as int
-    reads node.repr
-  {
-    Index(SubRepr(node, 0, newnchildren) + {node.pivots, node.children}, node.height, newnchildren as uint64, node.pivots, node.children)
-  }
+  // function method IndexPrefix(node: Node, newnchildren: int) : (result: Node)
+  //   requires WFShape(node)
+  //   requires node.Index?
+  //   requires 1 < node.nchildren
+  //   requires 0 <= newnchildren <= node.nchildren as int
+  //   reads node.repr
+  // {
+  //   Index(SubRepr(node, 0, newnchildren) + {node.pivots, node.children}, node.height, newnchildren as uint64, node.pivots, node.children)
+  // }
 
-  lemma IndexPrefixPreservesWFShape(node: Node, newnchildren: int)
-    requires WFShape(node)
-    requires node.Index?
-    requires 1 < node.nchildren
-    requires 0 < newnchildren <= node.nchildren as int
-    ensures WFShape(IndexPrefix(node, newnchildren))
-    ensures newnchildren < node.nchildren as int ==> IndexPrefix(node, newnchildren).repr < node.repr
-  {
-    var pnode := IndexPrefix(node, newnchildren);
-    forall i: int, j: int | 0 <= i < j < pnode.nchildren as int
-      ensures DisjointSubtrees(pnode, i, j)
-    {
-      assert DisjointSubtrees(node, i, j);
-    }
-    SubReprFits(node, 0, newnchildren);
-  }
+  // lemma IndexPrefixPreservesWFShape(node: Node, newnchildren: int)
+  //   requires WFShape(node)
+  //   requires node.Index?
+  //   requires 1 < node.nchildren
+  //   requires 0 < newnchildren <= node.nchildren as int
+  //   ensures WFShape(IndexPrefix(node, newnchildren))
+  //   ensures newnchildren < node.nchildren as int ==> IndexPrefix(node, newnchildren).repr < node.repr
+  // {
+  //   var pnode := IndexPrefix(node, newnchildren);
+  //   forall i: int, j: int | 0 <= i < j < pnode.nchildren as int
+  //     ensures DisjointSubtrees(pnode, i, j)
+  //   {
+  //     assert DisjointSubtrees(node, i, j);
+  //   }
+  //   SubReprFits(node, 0, newnchildren);
+  // }
 
-  function WFShapeIndexPrefix(node: Node, newnchildren: int) : (result: Node)
-    requires WFShape(node)
-    requires node.Index?
-    requires 1 < node.nchildren
-    requires 0 < newnchildren <= node.nchildren as int
-    ensures WFShape(result)
-    reads node.repr
-  {
-    IndexPrefixPreservesWFShape(node, newnchildren);
-    IndexPrefix(node, newnchildren)
-  }
+  // function WFShapeIndexPrefix(node: Node, newnchildren: int) : (result: Node)
+  //   requires WFShape(node)
+  //   requires node.Index?
+  //   requires 1 < node.nchildren
+  //   requires 0 < newnchildren <= node.nchildren as int
+  //   ensures WFShape(result)
+  //   reads node.repr
+  // {
+  //   IndexPrefixPreservesWFShape(node, newnchildren);
+  //   IndexPrefix(node, newnchildren)
+  // }
   
-  function I(node: Node) : (result: BS.Node)
-    requires WFShape(node)
-    ensures node.Leaf? ==> result.Leaf?
-    ensures node.Leaf? ==> result.keys == node.keys[..node.nkeys];
-    ensures node.Leaf? ==> result.values == node.values[..node.nkeys];
-    ensures node.Index? ==> result.Index?
-    ensures node.Index? ==> result.pivots == node.pivots[..node.nchildren-1]
-    ensures node.Index? ==> |result.children| == node.nchildren as int
-    ensures node.Index? ==> forall i :: 0 <= i < node.nchildren ==>
-           result.children[i] == I(node.children[i])
-    reads node.repr
-    decreases node.repr
-  {
-    match node {
-      case Leaf(_, _, nkeys, keys, values) => BS.Leaf(keys[..nkeys], values[..nkeys])
-      case Index(repr, _, nchildren, pivots, children) =>
-        if nchildren == 1 then
-          BS.Index([], [I(children[0])])
-        else
-          IndexPrefixPreservesWFShape(node, node.nchildren as int - 1);
-          var imprefix := I(IndexPrefix(node, node.nchildren as int - 1));
-          var imlastchild := I(children[nchildren-1]);
-          BS.Index(imprefix.pivots + [pivots[nchildren-2]], imprefix.children + [imlastchild])
-    }
-  }
+  // function I(node: Node) : (result: BS.Node)
+  //   requires WFShape(node)
+  //   ensures node.Leaf? ==> result.Leaf?
+  //   ensures node.Leaf? ==> result.keys == node.keys[..node.nkeys];
+  //   ensures node.Leaf? ==> result.values == node.values[..node.nkeys];
+  //   ensures node.Index? ==> result.Index?
+  //   ensures node.Index? ==> result.pivots == node.pivots[..node.nchildren-1]
+  //   ensures node.Index? ==> |result.children| == node.nchildren as int
+  //   ensures node.Index? ==> forall i :: 0 <= i < node.nchildren ==>
+  //          result.children[i] == I(node.children[i])
+  //   reads node.repr
+  //   decreases node.repr
+  // {
+  //   match node {
+  //     case Leaf(_, _, nkeys, keys, values) => BS.Leaf(keys[..nkeys], values[..nkeys])
+  //     case Index(repr, _, nchildren, pivots, children) =>
+  //       if nchildren == 1 then
+  //         BS.Index([], [I(children[0])])
+  //       else
+  //         IndexPrefixPreservesWFShape(node, node.nchildren as int - 1);
+  //         var imprefix := I(IndexPrefix(node, node.nchildren as int - 1));
+  //         var imlastchild := I(children[nchildren-1]);
+  //         BS.Index(imprefix.pivots + [pivots[nchildren-2]], imprefix.children + [imlastchild])
+  //   }
+  // }
 
-  predicate {:opaque} BSWF(node: BS.Node)
-  {
-    BS.WF(node)
-  }
+  // predicate {:opaque} BSWF(node: BS.Node)
+  // {
+  //   BS.WF(node)
+  // }
 
-  lemma BSWFImpliesChildBSWF(node: BS.Node, childidx: int)
-    requires BSWF(node)
-    requires node.Index?
-    requires 0 <= childidx < |node.children|
-    ensures BSWF(node.children[childidx])
-  {
-    reveal_BSWF();
-  }
+  // lemma BSWFImpliesChildBSWF(node: BS.Node, childidx: int)
+  //   requires BSWF(node)
+  //   requires node.Index?
+  //   requires 0 <= childidx < |node.children|
+  //   ensures BSWF(node.children[childidx])
+  // {
+  //   reveal_BSWF();
+  // }
   
-  function {:opaque} BSSubIndex(node: BS.Node, from: int, to: int) : BS.Node
-    requires BSWF(node)
-    requires node.Index?
-    requires 0 <= from < to <= |node.children|
-  {
-    reveal_BSWF();
-    BS.SubIndex(node, from, to)
-  }
+  // function {:opaque} BSSubIndex(node: BS.Node, from: int, to: int) : BS.Node
+  //   requires BSWF(node)
+  //   requires node.Index?
+  //   requires 0 <= from < to <= |node.children|
+  // {
+  //   reveal_BSWF();
+  //   BS.SubIndex(node, from, to)
+  // }
 
-  function {:opaque} BSInterpretation(node: BS.Node) : map<Key, Value>
-    requires BSWF(node)
-  {
-    reveal_BSWF();
-    BS.Interpretation(node)
-  }
+  // function {:opaque} BSInterpretation(node: BS.Node) : map<Key, Value>
+  //   requires BSWF(node)
+  // {
+  //   reveal_BSWF();
+  //   BS.Interpretation(node)
+  // }
   
-  function {:opaque} BSInterpretationOfChild(node: BS.Node, childidx: int) : map<Key, Value>
-    requires BSWF(node)
-    requires node.Index?
-    requires 0 <= childidx < |node.children|
-  {
-    reveal_BSWF();
-    BS.Interpretation(node.children[childidx])
-  }
+  // function {:opaque} BSInterpretationOfChild(node: BS.Node, childidx: int) : map<Key, Value>
+  //   requires BSWF(node)
+  //   requires node.Index?
+  //   requires 0 <= childidx < |node.children|
+  // {
+  //   reveal_BSWF();
+  //   BS.Interpretation(node.children[childidx])
+  // }
 
-  function {:opaque} BSAllKeys(node: BS.Node) : set<Key>
-  {
-    BS.AllKeys(node)
-  }
+  // function {:opaque} BSAllKeys(node: BS.Node) : set<Key>
+  // {
+  //   BS.AllKeys(node)
+  // }
   
-  function {:opaque} BSAllKeysOfChild(node: BS.Node, childidx: int) : set<Key>
-    requires node.Index?
-    requires 0 <= childidx < |node.children|
-  {
-    BS.AllKeys(node.children[childidx])
-  }
+  // function {:opaque} BSAllKeysOfChild(node: BS.Node, childidx: int) : set<Key>
+  //   requires node.Index?
+  //   requires 0 <= childidx < |node.children|
+  // {
+  //   BS.AllKeys(node.children[childidx])
+  // }
 
-  predicate {:opaque} BSSplitLeaf(oldleaf: BS.Node, leftleaf: BS.Node, rightleaf: BS.Node, wit: Key, pivot: Key)
-  {
-    BS.SplitLeaf(oldleaf, leftleaf, rightleaf, wit, pivot)
-  }
+  // predicate {:opaque} BSSplitLeaf(oldleaf: BS.Node, leftleaf: BS.Node, rightleaf: BS.Node, wit: Key, pivot: Key)
+  // {
+  //   BS.SplitLeaf(oldleaf, leftleaf, rightleaf, wit, pivot)
+  // }
 
-  predicate {:opaque} BSSplitIndex(oldleaf: BS.Node, leftleaf: BS.Node, rightleaf: BS.Node, wit: Key, pivot: Key)
-  {
-    BS.SplitIndex(oldleaf, leftleaf, rightleaf, wit, pivot)
-  }
+  // predicate {:opaque} BSSplitIndex(oldleaf: BS.Node, leftleaf: BS.Node, rightleaf: BS.Node, wit: Key, pivot: Key)
+  // {
+  //   BS.SplitIndex(oldleaf, leftleaf, rightleaf, wit, pivot)
+  // }
 
-  predicate {:opaque} BSSplitNode(oldleaf: BS.Node, leftleaf: BS.Node, rightleaf: BS.Node, wit: Key, pivot: Key)
-  {
-    BS.SplitNode(oldleaf, leftleaf, rightleaf, wit, pivot)
-  }
+  // predicate {:opaque} BSSplitNode(oldleaf: BS.Node, leftleaf: BS.Node, rightleaf: BS.Node, wit: Key, pivot: Key)
+  // {
+  //   BS.SplitNode(oldleaf, leftleaf, rightleaf, wit, pivot)
+  // }
 
-  predicate {:opaque} BSSplitChildOfIndex(oldindex: BS.Node, newindex: BS.Node, childidx: int, wit: Key)
-    requires oldindex.Index?
-    requires 0 <= childidx < |oldindex.children|
-  {
-    BS.SplitChildOfIndex(oldindex, newindex, childidx, wit)
-  }
+  // predicate {:opaque} BSSplitChildOfIndex(oldindex: BS.Node, newindex: BS.Node, childidx: int, wit: Key)
+  //   requires oldindex.Index?
+  //   requires 0 <= childidx < |oldindex.children|
+  // {
+  //   BS.SplitChildOfIndex(oldindex, newindex, childidx, wit)
+  // }
 
-  function {:opaque} BSInsertLeaf(leaf: BS.Node, key: Key, value: Value) : (result: BS.Node)
-    requires leaf.Leaf?
-    requires BSWF(leaf)
-  {
-    reveal_BSWF();
-    BS.InsertLeaf(leaf, key, value)
-  }
+  // function {:opaque} BSInsertLeaf(leaf: BS.Node, key: Key, value: Value) : (result: BS.Node)
+  //   requires leaf.Leaf?
+  //   requires BSWF(leaf)
+  // {
+  //   reveal_BSWF();
+  //   BS.InsertLeaf(leaf, key, value)
+  // }
 
-  function {:opaque} BSChildFor(node: BS.Node, key: Key) : (childidx: int)
-    requires node.Index?
-    requires BSWF(node)
-    ensures 0 <= childidx < |node.children|
-  {
-    reveal_BSWF();
-    BS.Keys.LargestLte(node.pivots, key) + 1
-  }
+  // function {:opaque} BSChildFor(node: BS.Node, key: Key) : (childidx: int)
+  //   requires node.Index?
+  //   requires BSWF(node)
+  //   ensures 0 <= childidx < |node.children|
+  // {
+  //   reveal_BSWF();
+  //   BS.Keys.LargestLte(node.pivots, key) + 1
+  // }
   
-  lemma IndexPrefixIsSubIndex(node: Node, newnchildren: int)
-    requires WFShape(node)
-    requires BSWF(I(node))
-    requires node.Index?
-    requires 1 < node.nchildren
-    requires 0 < newnchildren <= node.nchildren as int
-    ensures I(WFShapeIndexPrefix(node, newnchildren)) == BSSubIndex(I(node), 0, newnchildren)
-  {
-    reveal_BSSubIndex();
-  }
+  // lemma IndexPrefixIsSubIndex(node: Node, newnchildren: int)
+  //   requires WFShape(node)
+  //   requires BSWF(I(node))
+  //   requires node.Index?
+  //   requires 1 < node.nchildren
+  //   requires 0 < newnchildren <= node.nchildren as int
+  //   ensures I(WFShapeIndexPrefix(node, newnchildren)) == BSSubIndex(I(node), 0, newnchildren)
+  // {
+  //   reveal_BSSubIndex();
+  // }
     
-  method QueryLeaf(node: Node, needle: Key) returns (result: BS.QueryResult)
-    requires WFShape(node)
-    requires BSWF(I(node))
-    requires node.Leaf?
-    ensures needle in BSInterpretation(I(node)) ==> result == BS.Found(BSInterpretation(I(node))[needle])
-    ensures needle !in BSInterpretation(I(node)) ==> result == BS.NotFound
-    decreases node.height, 0
-  {
-    reveal_BSWF();
-    reveal_BSInterpretation();
-    var posplus1: uint64 := BS.Keys.ArrayLargestLtePlus1(node.keys, 0, node.nkeys, needle);
-    if 1 <= posplus1 && node.keys[posplus1-1] == needle {
-      result := BS.Found(node.values[posplus1-1]);
-    } else {
-      result := BS.NotFound;
-    }
-  }
+  // method QueryLeaf(node: Node, needle: Key) returns (result: BS.QueryResult)
+  //   requires WFShape(node)
+  //   requires BSWF(I(node))
+  //   requires node.Leaf?
+  //   ensures needle in BSInterpretation(I(node)) ==> result == BS.Found(BSInterpretation(I(node))[needle])
+  //   ensures needle !in BSInterpretation(I(node)) ==> result == BS.NotFound
+  //   decreases node.height, 0
+  // {
+  //   reveal_BSWF();
+  //   reveal_BSInterpretation();
+  //   var posplus1: uint64 := BS.Keys.ArrayLargestLtePlus1(node.keys, 0, node.nkeys, needle);
+  //   if 1 <= posplus1 && node.keys[posplus1-1] == needle {
+  //     result := BS.Found(node.values[posplus1-1]);
+  //   } else {
+  //     result := BS.NotFound;
+  //   }
+  // }
 
-  method QueryIndex(node: Node, needle: Key) returns (result: BS.QueryResult)
-    requires WFShape(node)
-    requires BSWF(I(node))
-    requires node.Index?
-    ensures needle in BSInterpretation(I(node)) ==> result == BS.Found(BSInterpretation(I(node))[needle])
-    ensures needle !in BSInterpretation(I(node)) ==> result == BS.NotFound
-    decreases node.height, 0
-  {
-    reveal_BSWF();
-    reveal_BSInterpretation();
-    reveal_BSAllKeys();
-    reveal_BSAllKeysOfChild();
-    reveal_BSInterpretationOfChild();
-    var posplus1 := BS.Keys.ArrayLargestLtePlus1(node.pivots, 0, node.nchildren-1, needle);
-    result := Query(node.children[posplus1], needle);
+  // method QueryIndex(node: Node, needle: Key) returns (result: BS.QueryResult)
+  //   requires WFShape(node)
+  //   requires BSWF(I(node))
+  //   requires node.Index?
+  //   ensures needle in BSInterpretation(I(node)) ==> result == BS.Found(BSInterpretation(I(node))[needle])
+  //   ensures needle !in BSInterpretation(I(node)) ==> result == BS.NotFound
+  //   decreases node.height, 0
+  // {
+  //   reveal_BSWF();
+  //   reveal_BSInterpretation();
+  //   reveal_BSAllKeys();
+  //   reveal_BSAllKeysOfChild();
+  //   reveal_BSInterpretationOfChild();
+  //   var posplus1 := BS.Keys.ArrayLargestLtePlus1(node.pivots, 0, node.nchildren-1, needle);
+  //   result := Query(node.children[posplus1], needle);
 
-    if needle !in BSInterpretation(I(node)) {
-      if needle !in BSAllKeys(I(node)) {
-        assert needle !in BSAllKeysOfChild(I(node), posplus1 as int);
-      }
-      assert needle !in BSInterpretationOfChild(I(node), posplus1 as int);
-    }
-  }
+  //   if needle !in BSInterpretation(I(node)) {
+  //     if needle !in BSAllKeys(I(node)) {
+  //       assert needle !in BSAllKeysOfChild(I(node), posplus1 as int);
+  //     }
+  //     assert needle !in BSInterpretationOfChild(I(node), posplus1 as int);
+  //   }
+  // }
 
-  method Query(node: Node, needle: Key) returns (result: BS.QueryResult)
-    requires WFShape(node)
-    requires BSWF(I(node))
-    ensures needle in BSInterpretation(I(node)) ==> result == BS.Found(BSInterpretation(I(node))[needle])
-    ensures needle !in BSInterpretation(I(node)) ==> result == BS.NotFound
-    decreases node.height, 1
-  {
-    match node {
-      case Leaf(_, _, _, _, _) => result := QueryLeaf(node, needle);
-      case Index(_, _, _, _, _) => result := QueryIndex(node, needle);
-    }
-  }
+  // method Query(node: Node, needle: Key) returns (result: BS.QueryResult)
+  //   requires WFShape(node)
+  //   requires BSWF(I(node))
+  //   ensures needle in BSInterpretation(I(node)) ==> result == BS.Found(BSInterpretation(I(node))[needle])
+  //   ensures needle !in BSInterpretation(I(node)) ==> result == BS.NotFound
+  //   decreases node.height, 1
+  // {
+  //   match node {
+  //     case Leaf(_, _, _, _, _) => result := QueryLeaf(node, needle);
+  //     case Index(_, _, _, _, _) => result := QueryIndex(node, needle);
+  //   }
+  // }
 
-  predicate method Full(node: Node)
-    requires !node.NotInUse?
-  {
-    match node {
-      case Leaf(_, _, nkeys, _, _) => nkeys == MaxKeysPerLeaf()
-      case Index(_, _, nchildren, _, _) => nchildren == MaxChildren()
-    }
-  }
+  // predicate method Full(node: Node)
+  //   requires !node.NotInUse?
+  // {
+  //   match node {
+  //     case Leaf(_, _, nkeys, _, _) => nkeys == MaxKeysPerLeaf()
+  //     case Index(_, _, nchildren, _, _) => nchildren == MaxChildren()
+  //   }
+  // }
 
-  method SplitLeaf(node: Node) returns (left: Node, right: Node, ghost wit: Key, pivot: Key)
-    requires WFShape(node)
-    requires BSWF(I(node))
-    requires node.Leaf?
-    requires Full(node)
-    ensures WFShape(left)
-    ensures WFShape(right)
-    ensures BSSplitLeaf(I(node), I(left), I(right), wit, pivot)
-    ensures left.Leaf?
-    ensures right.Leaf?
-    ensures left.keys == node.keys
-    ensures left.values == node.values
-    ensures fresh(right.keys)
-    ensures fresh(right.values)
-  {
-    var rightkeys := new Key[MaxKeysPerLeaf()](_ => DefaultKey());
-    var rightvalues := new Value[MaxKeysPerLeaf()](_ => DefaultValue());
-    var boundary := node.nkeys / 2;
-    Arrays.Memcpy(rightkeys, 0, node.keys[boundary..node.nkeys]); // FIXME: remove conversion to seq
-    Arrays.Memcpy(rightvalues, 0, node.values[boundary..node.nkeys]); // FIXME: remove conversion to seq
-    left := Leaf(node.repr, 0, boundary, node.keys, node.values);
-    right := Leaf({rightkeys, rightvalues}, 0, node.nkeys - boundary, rightkeys, rightvalues);
-    wit := left.keys[0];
-    pivot := right.keys[0];
+  // method SplitLeaf(node: Node) returns (left: Node, right: Node, ghost wit: Key, pivot: Key)
+  //   requires WFShape(node)
+  //   requires BSWF(I(node))
+  //   requires node.Leaf?
+  //   requires Full(node)
+  //   ensures WFShape(left)
+  //   ensures WFShape(right)
+  //   ensures BSSplitLeaf(I(node), I(left), I(right), wit, pivot)
+  //   ensures left.Leaf?
+  //   ensures right.Leaf?
+  //   ensures left.keys == node.keys
+  //   ensures left.values == node.values
+  //   ensures fresh(right.keys)
+  //   ensures fresh(right.values)
+  // {
+  //   var rightkeys := new Key[MaxKeysPerLeaf()](_ => DefaultKey());
+  //   var rightvalues := new Value[MaxKeysPerLeaf()](_ => DefaultValue());
+  //   var boundary := node.nkeys / 2;
+  //   Arrays.Memcpy(rightkeys, 0, node.keys[boundary..node.nkeys]); // FIXME: remove conversion to seq
+  //   Arrays.Memcpy(rightvalues, 0, node.values[boundary..node.nkeys]); // FIXME: remove conversion to seq
+  //   left := Leaf(node.repr, 0, boundary, node.keys, node.values);
+  //   right := Leaf({rightkeys, rightvalues}, 0, node.nkeys - boundary, rightkeys, rightvalues);
+  //   wit := left.keys[0];
+  //   pivot := right.keys[0];
     
-    BS.Keys.reveal_IsStrictlySorted();
-    reveal_BSSplitLeaf();
-  }
+  //   BS.Keys.reveal_IsStrictlySorted();
+  //   reveal_BSSplitLeaf();
+  // }
 
-  method SubIndex(node: Node, from: uint64, to: uint64) returns (subnode: Node)
-    requires WFShape(node)
-    requires BSWF(I(node))
-    requires node.Index?
-    requires 1 < node.nchildren
-    requires 0 <= from < to <= node.nchildren
-    ensures WFShape(subnode)
-    ensures subnode.Index?
-    ensures subnode.height == node.height
-    ensures I(subnode) == BSSubIndex(I(node), from as int, to as int)
-    ensures subnode.repr == SubRepr(node, from as int, to as int) + {subnode.pivots, subnode.children}
-    ensures fresh(subnode.pivots)
-    ensures fresh(subnode.children)
-  {
-    var subnchildren := to - from;
-    var subpivots := new Key[MaxChildren()-1]
-      (i
-      requires 0 <= i <= (MaxChildren()-1) as int
-      reads node.pivots
-      =>
-      if i < subnchildren as int - 1 then node.pivots[from as int + i]
-      else DefaultKey());
-    var subchildren := new Node[MaxChildren()]
-      (i
-      requires 0 <= i <= MaxChildren() as int
-      reads node.children
-      =>
-      if i < subnchildren as int then node.children[from as int + i]
-      else NotInUse);
-    ghost var subrepr := SubRepr(node, from as int, to as int) + {subpivots, subchildren};
-    subnode := Index(subrepr, node.height, subnchildren, subpivots, subchildren);
+  // method SubIndex(node: Node, from: uint64, to: uint64) returns (subnode: Node)
+  //   requires WFShape(node)
+  //   requires BSWF(I(node))
+  //   requires node.Index?
+  //   requires 1 < node.nchildren
+  //   requires 0 <= from < to <= node.nchildren
+  //   ensures WFShape(subnode)
+  //   ensures subnode.Index?
+  //   ensures subnode.height == node.height
+  //   ensures I(subnode) == BSSubIndex(I(node), from as int, to as int)
+  //   ensures subnode.repr == SubRepr(node, from as int, to as int) + {subnode.pivots, subnode.children}
+  //   ensures fresh(subnode.pivots)
+  //   ensures fresh(subnode.children)
+  // {
+  //   var subnchildren := to - from;
+  //   var subpivots := new Key[MaxChildren()-1]
+  //     (i
+  //     requires 0 <= i <= (MaxChildren()-1) as int
+  //     reads node.pivots
+  //     =>
+  //     if i < subnchildren as int - 1 then node.pivots[from as int + i]
+  //     else DefaultKey());
+  //   var subchildren := new Node[MaxChildren()]
+  //     (i
+  //     requires 0 <= i <= MaxChildren() as int
+  //     reads node.children
+  //     =>
+  //     if i < subnchildren as int then node.children[from as int + i]
+  //     else NotInUse);
+  //   ghost var subrepr := SubRepr(node, from as int, to as int) + {subpivots, subchildren};
+  //   subnode := Index(subrepr, node.height, subnchildren, subpivots, subchildren);
 
-    SubReprFits(node, from as int, to as int);
-    forall i, j | 0 <= i < j < subnode.nchildren as int
-      ensures DisjointSubtrees(subnode, i, j)
-    {
-      assert subnode.children[i] == node.children[from as int + i];
-      assert subnode.children[j] == node.children[from as int + j];
-      assert DisjointSubtrees(node, from as int + i, from as int + j);
-    }
+  //   SubReprFits(node, from as int, to as int);
+  //   forall i, j | 0 <= i < j < subnode.nchildren as int
+  //     ensures DisjointSubtrees(subnode, i, j)
+  //   {
+  //     assert subnode.children[i] == node.children[from as int + i];
+  //     assert subnode.children[j] == node.children[from as int + j];
+  //     assert DisjointSubtrees(node, from as int + i, from as int + j);
+  //   }
 
-    ghost var inode := I(node);
-    ghost var isubnode := I(subnode);
-    assert subnode.pivots[..subnode.nchildren-1] == node.pivots[from..to-1];
-    assert isubnode.pivots == inode.pivots[from..to-1];
-    assert isubnode.children == inode.children[from..to];
-    reveal_BSWF();
-    reveal_BSSubIndex();
-  }
+  //   ghost var inode := I(node);
+  //   ghost var isubnode := I(subnode);
+  //   assert subnode.pivots[..subnode.nchildren-1] == node.pivots[from..to-1];
+  //   assert isubnode.pivots == inode.pivots[from..to-1];
+  //   assert isubnode.children == inode.children[from..to];
+  //   reveal_BSWF();
+  //   reveal_BSSubIndex();
+  // }
 
   
-  method SplitIndex(node: Node) returns (left: Node, right: Node, ghost wit: Key, pivot: Key)
-    requires WFShape(node)
-    requires BSWF(I(node))
-    requires node.Index?
-    requires Full(node)
-    ensures WFShape(left)
-    ensures WFShape(right)
-    ensures left.Index?
-    ensures right.Index?
-    ensures left.height == node.height
-    ensures right.height == node.height
-    ensures BSSplitIndex(I(node), I(left), I(right), wit, pivot)
-    ensures left.pivots == node.pivots
-    ensures left.children == node.children
-    ensures fresh(right.pivots)
-    ensures fresh(right.children)
-    ensures left.repr !! right.repr
-    ensures left.repr <= node.repr
-    ensures right.repr <= node.repr + {right.pivots, right.children}
-  {
-    var boundary := node.nchildren/2;
-    left := IndexPrefix(node, boundary as int);
-    right := SubIndex(node, boundary, node.nchildren);
-    reveal_BSWF();
-    if node.children[0].Leaf? {
-      wit := node.children[0].keys[0];
-    } else {
-      wit :| wit in BS.AllKeys(I(node.children[0]));
-    }
-    pivot := node.pivots[boundary-1];
+  // method SplitIndex(node: Node) returns (left: Node, right: Node, ghost wit: Key, pivot: Key)
+  //   requires WFShape(node)
+  //   requires BSWF(I(node))
+  //   requires node.Index?
+  //   requires Full(node)
+  //   ensures WFShape(left)
+  //   ensures WFShape(right)
+  //   ensures left.Index?
+  //   ensures right.Index?
+  //   ensures left.height == node.height
+  //   ensures right.height == node.height
+  //   ensures BSSplitIndex(I(node), I(left), I(right), wit, pivot)
+  //   ensures left.pivots == node.pivots
+  //   ensures left.children == node.children
+  //   ensures fresh(right.pivots)
+  //   ensures fresh(right.children)
+  //   ensures left.repr !! right.repr
+  //   ensures left.repr <= node.repr
+  //   ensures right.repr <= node.repr + {right.pivots, right.children}
+  // {
+  //   var boundary := node.nchildren/2;
+  //   left := IndexPrefix(node, boundary as int);
+  //   right := SubIndex(node, boundary, node.nchildren);
+  //   reveal_BSWF();
+  //   if node.children[0].Leaf? {
+  //     wit := node.children[0].keys[0];
+  //   } else {
+  //     wit :| wit in BS.AllKeys(I(node.children[0]));
+  //   }
+  //   pivot := node.pivots[boundary-1];
     
-    IndexPrefixPreservesWFShape(node, boundary as int);
-    IndexPrefixIsSubIndex(node, boundary as int);
-    BS.SubIndexPreservesWF(I(node), 0, boundary as int);
-    BS.SubIndexPreservesWF(I(node), boundary as int, node.nchildren as int);
-    SubReprsDisjoint(node, 0, boundary as int, boundary as int, node.nchildren as int);
-    SubReprFits(node, 0, boundary as int);
-    SubReprFits(node, boundary as int, node.nchildren as int);
+  //   IndexPrefixPreservesWFShape(node, boundary as int);
+  //   IndexPrefixIsSubIndex(node, boundary as int);
+  //   BS.SubIndexPreservesWF(I(node), 0, boundary as int);
+  //   BS.SubIndexPreservesWF(I(node), boundary as int, node.nchildren as int);
+  //   SubReprsDisjoint(node, 0, boundary as int, boundary as int, node.nchildren as int);
+  //   SubReprFits(node, 0, boundary as int);
+  //   SubReprFits(node, boundary as int, node.nchildren as int);
 
-    reveal_BSSubIndex();
-    reveal_BSSplitIndex();
+  //   reveal_BSSubIndex();
+  //   reveal_BSSplitIndex();
 
-    assert BS.SplitIndex(I(node), I(left), I(right), wit, pivot);
-  }
+  //   assert BS.SplitIndex(I(node), I(left), I(right), wit, pivot);
+  // }
 
-  method SplitNode(node: Node) returns (left: Node, right: Node, ghost wit: Key, pivot: Key)
-    requires WFShape(node)
-    requires BSWF(I(node))
-    requires Full(node)
-    ensures WFShape(left)
-    ensures WFShape(right)
-    ensures left.height == node.height
-    ensures right.height == node.height
-    ensures BSSplitNode(I(node), I(left), I(right), wit, pivot)
-    ensures left.repr <= node.repr
-    ensures fresh(right.repr - node.repr)
-    ensures left.repr !! right.repr
-  {
-    reveal_BSSplitNode();
-    reveal_BSSplitLeaf();
-    reveal_BSSplitIndex();
-    if node.Leaf? {
-      left, right, wit, pivot := SplitLeaf(node);
-    } else {
-      left, right, wit, pivot := SplitIndex(node);
-    }
-  }
+  // method SplitNode(node: Node) returns (left: Node, right: Node, ghost wit: Key, pivot: Key)
+  //   requires WFShape(node)
+  //   requires BSWF(I(node))
+  //   requires Full(node)
+  //   ensures WFShape(left)
+  //   ensures WFShape(right)
+  //   ensures left.height == node.height
+  //   ensures right.height == node.height
+  //   ensures BSSplitNode(I(node), I(left), I(right), wit, pivot)
+  //   ensures left.repr <= node.repr
+  //   ensures fresh(right.repr - node.repr)
+  //   ensures left.repr !! right.repr
+  // {
+  //   reveal_BSSplitNode();
+  //   reveal_BSSplitLeaf();
+  //   reveal_BSSplitIndex();
+  //   if node.Leaf? {
+  //     left, right, wit, pivot := SplitLeaf(node);
+  //   } else {
+  //     left, right, wit, pivot := SplitIndex(node);
+  //   }
+  // }
 
-  lemma SplitChildOfIndexPreservesDisjointReprs(oldchildren: seq<Node>, childidx: int, left: Node, right: Node)
-    requires forall i :: 0 <= i < |oldchildren| ==> !oldchildren[i].NotInUse?
-    requires 0 <= childidx < |oldchildren|
-    requires !left.NotInUse?
-    requires !right.NotInUse?
-    requires forall i, j :: 0 <= i < j < |oldchildren| ==> oldchildren[i].repr !! oldchildren[j].repr
-    requires left.repr !! right.repr
-    requires left.repr <= oldchildren[childidx].repr
-    requires forall i :: 0 <= i < |oldchildren| && i != childidx ==> right.repr !! oldchildren[i].repr
-    ensures forall i :: 0 <= i < |Seq.replace1with2(oldchildren, left, right, childidx)| ==> !Seq.replace1with2(oldchildren, left, right, childidx)[i].NotInUse?
-    ensures forall i, j :: 0 <= i < j < |oldchildren|+1 ==> Seq.replace1with2(oldchildren, left, right, childidx)[i].repr !! Seq.replace1with2(oldchildren, left, right, childidx)[j].repr
-  {
-    var newchildren := Seq.replace1with2(oldchildren, left, right, childidx);
-    forall i | 0 <= i < |newchildren|
-      ensures !newchildren[i].NotInUse?
-    {
-      if i < childidx {
-      } else if i == childidx {
-      } else if i == childidx + 1 {
-      } else {
-        assert newchildren[i] == oldchildren[i-1];
-      }
-    }
+  // lemma SplitChildOfIndexPreservesDisjointReprs(oldchildren: seq<Node>, childidx: int, left: Node, right: Node)
+  //   requires forall i :: 0 <= i < |oldchildren| ==> !oldchildren[i].NotInUse?
+  //   requires 0 <= childidx < |oldchildren|
+  //   requires !left.NotInUse?
+  //   requires !right.NotInUse?
+  //   requires forall i, j :: 0 <= i < j < |oldchildren| ==> oldchildren[i].repr !! oldchildren[j].repr
+  //   requires left.repr !! right.repr
+  //   requires left.repr <= oldchildren[childidx].repr
+  //   requires forall i :: 0 <= i < |oldchildren| && i != childidx ==> right.repr !! oldchildren[i].repr
+  //   ensures forall i :: 0 <= i < |Seq.replace1with2(oldchildren, left, right, childidx)| ==> !Seq.replace1with2(oldchildren, left, right, childidx)[i].NotInUse?
+  //   ensures forall i, j :: 0 <= i < j < |oldchildren|+1 ==> Seq.replace1with2(oldchildren, left, right, childidx)[i].repr !! Seq.replace1with2(oldchildren, left, right, childidx)[j].repr
+  // {
+  //   var newchildren := Seq.replace1with2(oldchildren, left, right, childidx);
+  //   forall i | 0 <= i < |newchildren|
+  //     ensures !newchildren[i].NotInUse?
+  //   {
+  //     if i < childidx {
+  //     } else if i == childidx {
+  //     } else if i == childidx + 1 {
+  //     } else {
+  //       assert newchildren[i] == oldchildren[i-1];
+  //     }
+  //   }
 
-    forall i: int, j: int | 0 <= i < j < |newchildren|
-      ensures newchildren[i].repr !! newchildren[j].repr
-    {
-      if                           j <  childidx       {
-      } else if                    j == childidx       {
-      } else if i < childidx     && j == childidx+1     {
-      } else if i == childidx    && j == childidx+1     {
-      } else if i < childidx     &&      childidx+1 < j {
-        assert newchildren[j] == oldchildren[j-1];
-      } else if i == childidx    &&      childidx+1 < j {
-        assert newchildren[j] == oldchildren[j-1];
-      } else if i == childidx+1  &&      childidx+1 < j {
-        assert newchildren[j] == oldchildren[j-1];
-      } else {
-        assert newchildren[i] == oldchildren[i-1];
-        assert newchildren[j] == oldchildren[j-1];
-      }
-    }
-  }
+  //   forall i: int, j: int | 0 <= i < j < |newchildren|
+  //     ensures newchildren[i].repr !! newchildren[j].repr
+  //   {
+  //     if                           j <  childidx       {
+  //     } else if                    j == childidx       {
+  //     } else if i < childidx     && j == childidx+1     {
+  //     } else if i == childidx    && j == childidx+1     {
+  //     } else if i < childidx     &&      childidx+1 < j {
+  //       assert newchildren[j] == oldchildren[j-1];
+  //     } else if i == childidx    &&      childidx+1 < j {
+  //       assert newchildren[j] == oldchildren[j-1];
+  //     } else if i == childidx+1  &&      childidx+1 < j {
+  //       assert newchildren[j] == oldchildren[j-1];
+  //     } else {
+  //       assert newchildren[i] == oldchildren[i-1];
+  //       assert newchildren[j] == oldchildren[j-1];
+  //     }
+  //   }
+  // }
   
-  method SplitChildOfIndexHelper(node: Node, childidx: uint64) returns (newnode: Node, ghost wit: Key)
-    requires WFShape(node)
-    requires BSWF(I(node))
-    requires node.Index?
-    requires !Full(node)
-    requires 0 <= childidx < node.nchildren
-    requires Full(node.children[childidx]);
-    ensures WFShape(newnode)
-    ensures newnode.Index?
-    ensures fresh(newnode.repr - node.repr)
-    ensures newnode.height == node.height
-    ensures newnode.pivots[..newnode.nchildren-1] == Seq.insert(old(node.pivots[..node.nchildren-1]), newnode.pivots[childidx], childidx as int)
-    ensures newnode.children[..newnode.nchildren] == Seq.replace1with2(old(node.children[..node.nchildren]), newnode.children[childidx], newnode.children[childidx+1], childidx as int)
-    ensures old(WFShape(node.children[childidx]))
-    ensures WFShape(newnode.children[childidx])
-    ensures WFShape(newnode.children[childidx+1])
-    ensures BSSplitNode(old(I(node.children[childidx])), I(newnode.children[childidx]), I(newnode.children[childidx+1]), wit, newnode.pivots[childidx])
-    modifies node.pivots, node.children
-  {
-    BSWFImpliesChildBSWF(I(node), childidx as int);
-    var left, right, wit', pivot := SplitNode(node.children[childidx]);
-    Arrays.replace1with2(node.children, node.nchildren, left, right, childidx);
-    Arrays.Insert(node.pivots, node.nchildren-1, pivot, childidx);
-    newnode := Index(node.repr + right.repr, node.height, node.nchildren + 1, node.pivots, node.children);
-    wit := wit';
+  // method SplitChildOfIndexHelper(node: Node, childidx: uint64) returns (newnode: Node, ghost wit: Key)
+  //   requires WFShape(node)
+  //   requires BSWF(I(node))
+  //   requires node.Index?
+  //   requires !Full(node)
+  //   requires 0 <= childidx < node.nchildren
+  //   requires Full(node.children[childidx]);
+  //   ensures WFShape(newnode)
+  //   ensures newnode.Index?
+  //   ensures fresh(newnode.repr - node.repr)
+  //   ensures newnode.height == node.height
+  //   ensures newnode.pivots[..newnode.nchildren-1] == Seq.insert(old(node.pivots[..node.nchildren-1]), newnode.pivots[childidx], childidx as int)
+  //   ensures newnode.children[..newnode.nchildren] == Seq.replace1with2(old(node.children[..node.nchildren]), newnode.children[childidx], newnode.children[childidx+1], childidx as int)
+  //   ensures old(WFShape(node.children[childidx]))
+  //   ensures WFShape(newnode.children[childidx])
+  //   ensures WFShape(newnode.children[childidx+1])
+  //   ensures BSSplitNode(old(I(node.children[childidx])), I(newnode.children[childidx]), I(newnode.children[childidx+1]), wit, newnode.pivots[childidx])
+  //   modifies node.pivots, node.children
+  // {
+  //   BSWFImpliesChildBSWF(I(node), childidx as int);
+  //   var left, right, wit', pivot := SplitNode(node.children[childidx]);
+  //   Arrays.replace1with2(node.children, node.nchildren, left, right, childidx);
+  //   Arrays.Insert(node.pivots, node.nchildren-1, pivot, childidx);
+  //   newnode := Index(node.repr + right.repr, node.height, node.nchildren + 1, node.pivots, node.children);
+  //   wit := wit';
     
-    ghost var oldchildren := old(node.children[..node.nchildren]);
-    ghost var newchildren := newnode.children[..newnode.nchildren];
-    ghost var ichildidx := childidx as int;
-    assert newchildren == Seq.replace1with2(oldchildren, left, right, ichildidx);
+  //   ghost var oldchildren := old(node.children[..node.nchildren]);
+  //   ghost var newchildren := newnode.children[..newnode.nchildren];
+  //   ghost var ichildidx := childidx as int;
+  //   assert newchildren == Seq.replace1with2(oldchildren, left, right, ichildidx);
 
-    forall i: int, j: int | 0 <= i < j < newnode.nchildren as int
-      ensures DisjointSubtrees(newnode, i, j)
-    {
-      if                            j <  ichildidx {
-        assert old(DisjointSubtrees(node, i, j));
-      } else if                     j == ichildidx {
-        assert old(DisjointSubtrees(node, i, j));
-      } else if i < ichildidx     && j == ichildidx+1 {
-        assert old(DisjointSubtrees(node, i, j-1));
-      } else if i == ichildidx    && j == ichildidx+1 {
-        assert newnode.children[i] == left;
-        assert newnode.children[j] == right;
-      } else if i < ichildidx     &&      ichildidx+1 < j {
-        assert old(DisjointSubtrees(node, i, j-1));
-      } else if i == ichildidx    &&      ichildidx+1 < j {
-        assert old(DisjointSubtrees(node, i, j-1));
-      } else if i == ichildidx+1  &&      ichildidx+1 < j {
-        assert old(DisjointSubtrees(node, i-1, j-1));
-      } else {
-        assert old(DisjointSubtrees(node, i-1, j-1));
-      }
-    }
+  //   forall i: int, j: int | 0 <= i < j < newnode.nchildren as int
+  //     ensures DisjointSubtrees(newnode, i, j)
+  //   {
+  //     if                            j <  ichildidx {
+  //       assert old(DisjointSubtrees(node, i, j));
+  //     } else if                     j == ichildidx {
+  //       assert old(DisjointSubtrees(node, i, j));
+  //     } else if i < ichildidx     && j == ichildidx+1 {
+  //       assert old(DisjointSubtrees(node, i, j-1));
+  //     } else if i == ichildidx    && j == ichildidx+1 {
+  //       assert newnode.children[i] == left;
+  //       assert newnode.children[j] == right;
+  //     } else if i < ichildidx     &&      ichildidx+1 < j {
+  //       assert old(DisjointSubtrees(node, i, j-1));
+  //     } else if i == ichildidx    &&      ichildidx+1 < j {
+  //       assert old(DisjointSubtrees(node, i, j-1));
+  //     } else if i == ichildidx+1  &&      ichildidx+1 < j {
+  //       assert old(DisjointSubtrees(node, i-1, j-1));
+  //     } else {
+  //       assert old(DisjointSubtrees(node, i-1, j-1));
+  //     }
+  //   }
 
-    forall i | 0 <= i < newnode.nchildren
-      ensures !newchildren[i].NotInUse?
-      ensures newchildren[i].repr < newnode.repr
-      ensures newnode.pivots !in newchildren[i].repr
-      ensures newnode.children !in newchildren[i].repr
-      ensures WFShape(newchildren[i])
-    {
-      if i < childidx {
-        assert newchildren[i] == oldchildren[i];
-        assert WFShape(newchildren[i]) == old(WFShape(oldchildren[i]));
-      } else if i == childidx {
-        assert newchildren[i] == left;
-        assert WFShape(left);
-      } else if i == childidx + 1 {
-        assert newchildren[i] == right;
-        assert WFShape(right);
-      } else {
-        assert newchildren[i] == oldchildren[ichildidx := left][i-1];
-        assert WFShape(newchildren[i]) == old(WFShape(oldchildren[ichildidx := left][i-1]));
-      }
-    }
+  //   forall i | 0 <= i < newnode.nchildren
+  //     ensures !newchildren[i].NotInUse?
+  //     ensures newchildren[i].repr < newnode.repr
+  //     ensures newnode.pivots !in newchildren[i].repr
+  //     ensures newnode.children !in newchildren[i].repr
+  //     ensures WFShape(newchildren[i])
+  //   {
+  //     if i < childidx {
+  //       assert newchildren[i] == oldchildren[i];
+  //       assert WFShape(newchildren[i]) == old(WFShape(oldchildren[i]));
+  //     } else if i == childidx {
+  //       assert newchildren[i] == left;
+  //       assert WFShape(left);
+  //     } else if i == childidx + 1 {
+  //       assert newchildren[i] == right;
+  //       assert WFShape(right);
+  //     } else {
+  //       assert newchildren[i] == oldchildren[ichildidx := left][i-1];
+  //       assert WFShape(newchildren[i]) == old(WFShape(oldchildren[ichildidx := left][i-1]));
+  //     }
+  //   }
 
-    forall o | o in newnode.repr - node.repr
-      ensures fresh(o)
-    {
-      assert o in right.repr - node.repr;
-    }
+  //   forall o | o in newnode.repr - node.repr
+  //     ensures fresh(o)
+  //   {
+  //     assert o in right.repr - node.repr;
+  //   }
 
-  }
+  // }
   
-  lemma SplitChildOfIndexIsBSSplitChildOfIndex(oldnode: BS.Node, newnode: BS.Node, childidx: int, wit: Key)
-    requires BSWF(oldnode)
-    requires oldnode.Index?
-    requires newnode.Index?
-    requires 0 <= childidx < |oldnode.children|
-    requires |oldnode.pivots| == |oldnode.children|-1 // redundant, but necessary
-    requires |newnode.children| == |oldnode.children| + 1
-    requires |newnode.pivots| == |oldnode.pivots| + 1
-    requires newnode.pivots == Seq.insert(oldnode.pivots, newnode.pivots[childidx], childidx)
-    requires newnode.children == Seq.replace1with2(oldnode.children, newnode.children[childidx], newnode.children[childidx+1], childidx)
-    requires BSSplitNode(oldnode.children[childidx], newnode.children[childidx], newnode.children[childidx+1], wit, newnode.pivots[childidx])
-    ensures BSSplitChildOfIndex(oldnode, newnode, childidx, wit)
-  {
-    reveal_BSWF();
-    reveal_BSSplitNode();
-    reveal_BSSplitChildOfIndex();
-  }
+  // lemma SplitChildOfIndexIsBSSplitChildOfIndex(oldnode: BS.Node, newnode: BS.Node, childidx: int, wit: Key)
+  //   requires BSWF(oldnode)
+  //   requires oldnode.Index?
+  //   requires newnode.Index?
+  //   requires 0 <= childidx < |oldnode.children|
+  //   requires |oldnode.pivots| == |oldnode.children|-1 // redundant, but necessary
+  //   requires |newnode.children| == |oldnode.children| + 1
+  //   requires |newnode.pivots| == |oldnode.pivots| + 1
+  //   requires newnode.pivots == Seq.insert(oldnode.pivots, newnode.pivots[childidx], childidx)
+  //   requires newnode.children == Seq.replace1with2(oldnode.children, newnode.children[childidx], newnode.children[childidx+1], childidx)
+  //   requires BSSplitNode(oldnode.children[childidx], newnode.children[childidx], newnode.children[childidx+1], wit, newnode.pivots[childidx])
+  //   ensures BSSplitChildOfIndex(oldnode, newnode, childidx, wit)
+  // {
+  //   reveal_BSWF();
+  //   reveal_BSSplitNode();
+  //   reveal_BSSplitChildOfIndex();
+  // }
     
-  method SplitChildOfIndex(node: Node, childidx: uint64) returns (newnode: Node, ghost wit: Key)
-    requires WFShape(node)
-    requires BSWF(I(node))
-    requires node.Index?
-    requires !Full(node)
-    requires 0 <= childidx < node.nchildren
-    requires Full(node.children[childidx])
-    ensures WFShape(newnode)
-    ensures newnode.height == node.height
-    ensures fresh(newnode.repr - node.repr)
-    ensures BSSplitChildOfIndex(old(I(node)), I(newnode), childidx as int, wit)
-    modifies node.pivots, node.children
-  {
-    newnode, wit := SplitChildOfIndexHelper(node, childidx);
-    assert newnode.children[..newnode.nchildren] == Seq.replace1with2(old(node.children[..node.nchildren]), newnode.children[childidx], newnode.children[childidx+1], childidx as int);
+  // method SplitChildOfIndex(node: Node, childidx: uint64) returns (newnode: Node, ghost wit: Key)
+  //   requires WFShape(node)
+  //   requires BSWF(I(node))
+  //   requires node.Index?
+  //   requires !Full(node)
+  //   requires 0 <= childidx < node.nchildren
+  //   requires Full(node.children[childidx])
+  //   ensures WFShape(newnode)
+  //   ensures newnode.height == node.height
+  //   ensures fresh(newnode.repr - node.repr)
+  //   ensures BSSplitChildOfIndex(old(I(node)), I(newnode), childidx as int, wit)
+  //   modifies node.pivots, node.children
+  // {
+  //   newnode, wit := SplitChildOfIndexHelper(node, childidx);
+  //   assert newnode.children[..newnode.nchildren] == Seq.replace1with2(old(node.children[..node.nchildren]), newnode.children[childidx], newnode.children[childidx+1], childidx as int);
 
-    ghost var ioldnode := old(I(node));
-    ghost var inewnode := I(newnode);
-    ghost var replaced := Seq.replace1with2(ioldnode.children, inewnode.children[childidx], inewnode.children[childidx+1], childidx as int);
-    forall i | 0 <= i < |inewnode.children|
-      ensures inewnode.children[i] == replaced[i]
-    {
-      if i < childidx as int {
-      } else if i == childidx as int {
-      } else if i == childidx as int + 1 {
-      } else {
-        assert newnode.children[i] == old(node.children[i-1]);
-      }
-    }
-    SplitChildOfIndexIsBSSplitChildOfIndex(old(I(node)), I(newnode), childidx as int, wit);
-  }
+  //   ghost var ioldnode := old(I(node));
+  //   ghost var inewnode := I(newnode);
+  //   ghost var replaced := Seq.replace1with2(ioldnode.children, inewnode.children[childidx], inewnode.children[childidx+1], childidx as int);
+  //   forall i | 0 <= i < |inewnode.children|
+  //     ensures inewnode.children[i] == replaced[i]
+  //   {
+  //     if i < childidx as int {
+  //     } else if i == childidx as int {
+  //     } else if i == childidx as int + 1 {
+  //     } else {
+  //       assert newnode.children[i] == old(node.children[i-1]);
+  //     }
+  //   }
+  //   SplitChildOfIndexIsBSSplitChildOfIndex(old(I(node)), I(newnode), childidx as int, wit);
+  // }
 
-  method InsertLeaf(node: Node, key: Key, value: Value) returns (result: Node)
-    requires WFShape(node)
-    requires BSWF(I(node))
-    requires node.Leaf?
-    requires !Full(node)
-    ensures WFShape(result)
-    ensures result.repr == node.repr
-    ensures result.Leaf?
-    ensures BSWF(I(result))
-    ensures BSInterpretation(I(result)) == BSInterpretation(old(I(node)))[key := value]
-    ensures BSAllKeys(I(result)) <= old(BSAllKeys(I(node))) + {key}
-    modifies node.keys, node.values
-  {
-    reveal_BSWF();
-    reveal_BSInsertLeaf();
-    reveal_BSInterpretation();
+  // method InsertLeaf(node: Node, key: Key, value: Value) returns (result: Node)
+  //   requires WFShape(node)
+  //   requires BSWF(I(node))
+  //   requires node.Leaf?
+  //   requires !Full(node)
+  //   ensures WFShape(result)
+  //   ensures result.repr == node.repr
+  //   ensures result.Leaf?
+  //   ensures BSWF(I(result))
+  //   ensures BSInterpretation(I(result)) == BSInterpretation(old(I(node)))[key := value]
+  //   ensures BSAllKeys(I(result)) <= old(BSAllKeys(I(node))) + {key}
+  //   modifies node.keys, node.values
+  // {
+  //   reveal_BSWF();
+  //   reveal_BSInsertLeaf();
+  //   reveal_BSInterpretation();
     
-    var posplus1: uint64 := BS.Keys.ArrayLargestLtePlus1(node.keys, 0, node.nkeys, key);
-    if 1 <= posplus1 && node.keys[posplus1-1] == key {
-      node.values[posplus1-1] := value;
-      result := node;
-    } else {
-      Arrays.Insert(node.keys, node.nkeys, key, posplus1);
-      Arrays.Insert(node.values, node.nkeys, value, posplus1);
-      result := node.(nkeys := node.nkeys + 1);
-    }
-    assert I(result) == BSInsertLeaf(old(I(node)), key, value);
-    reveal_BSAllKeys();
-    BS.InsertLeafIsCorrect(old(I(node)), key, value);
-  }
+  //   var posplus1: uint64 := BS.Keys.ArrayLargestLtePlus1(node.keys, 0, node.nkeys, key);
+  //   if 1 <= posplus1 && node.keys[posplus1-1] == key {
+  //     node.values[posplus1-1] := value;
+  //     result := node;
+  //   } else {
+  //     Arrays.Insert(node.keys, node.nkeys, key, posplus1);
+  //     Arrays.Insert(node.values, node.nkeys, value, posplus1);
+  //     result := node.(nkeys := node.nkeys + 1);
+  //   }
+  //   assert I(result) == BSInsertLeaf(old(I(node)), key, value);
+  //   reveal_BSAllKeys();
+  //   BS.InsertLeafIsCorrect(old(I(node)), key, value);
+  // }
 
-  method InsertIndexChildIsNotFullHelper(node: Node, key: Key, value: Value, childidx: uint64) returns (result: Node)
-    requires WFShape(node)
-    requires BSWF(I(node))
-    requires node.Index?
-    requires childidx as int == BSChildFor(I(node), key)
-    requires BSWF(I(node).children[childidx])
-    requires !Full(node.children[childidx])
-    ensures WFShape(result)
-    ensures result.height == node.height
-    ensures fresh(result.repr - node.repr)
-    ensures result.Index?
-    ensures result.nchildren == node.nchildren
-    ensures result.pivots == node.pivots
-    ensures result.children == node.children
-    ensures forall i :: 0 <= i < result.nchildren && i != childidx ==> result.children[i] == old(node.children[i])
-    ensures BSWF(I(result.children[childidx]))
-    ensures BSInterpretation(I(result.children[childidx])) == old(BSInterpretation(I(node).children[childidx]))[key := value]
-    ensures BSAllKeys(I(result.children[childidx])) <= old(BSAllKeys(I(node.children[childidx]))) + {key}
-    ensures childidx < node.nchildren-1 ==> (forall key :: key in BSAllKeys(I(result.children[childidx])) ==> BS.Keys.lt(key, node.pivots[childidx]))
-    ensures BSWF(I(result))
-    ensures BSInterpretation(I(result)) == BSInterpretation(old(I(node)))[key := value]
-    modifies node.children, node.children[childidx].repr
-    decreases node.height, 0
-  {
-    reveal_BSWF();
-    node.children[childidx] := InsertNode(node.children[childidx], key, value);
-    result := node.(repr := node.repr + node.children[childidx].repr);
+  // method InsertIndexChildIsNotFullHelper(node: Node, key: Key, value: Value, childidx: uint64) returns (result: Node)
+  //   requires WFShape(node)
+  //   requires BSWF(I(node))
+  //   requires node.Index?
+  //   requires childidx as int == BSChildFor(I(node), key)
+  //   requires BSWF(I(node).children[childidx])
+  //   requires !Full(node.children[childidx])
+  //   ensures WFShape(result)
+  //   ensures result.height == node.height
+  //   ensures fresh(result.repr - node.repr)
+  //   ensures result.Index?
+  //   ensures result.nchildren == node.nchildren
+  //   ensures result.pivots == node.pivots
+  //   ensures result.children == node.children
+  //   ensures forall i :: 0 <= i < result.nchildren && i != childidx ==> result.children[i] == old(node.children[i])
+  //   ensures BSWF(I(result.children[childidx]))
+  //   ensures BSInterpretation(I(result.children[childidx])) == old(BSInterpretation(I(node).children[childidx]))[key := value]
+  //   ensures BSAllKeys(I(result.children[childidx])) <= old(BSAllKeys(I(node.children[childidx]))) + {key}
+  //   ensures childidx < node.nchildren-1 ==> (forall key :: key in BSAllKeys(I(result.children[childidx])) ==> BS.Keys.lt(key, node.pivots[childidx]))
+  //   ensures BSWF(I(result))
+  //   ensures BSInterpretation(I(result)) == BSInterpretation(old(I(node)))[key := value]
+  //   modifies node.children, node.children[childidx].repr
+  //   decreases node.height, 0
+  // {
+  //   reveal_BSWF();
+  //   node.children[childidx] := InsertNode(node.children[childidx], key, value);
+  //   result := node.(repr := node.repr + node.children[childidx].repr);
 
-    ghost var ichildidx := childidx as int;
-    forall i: int, j: int | 0 <= i < j < result.nchildren as int
-      ensures DisjointSubtrees(result, i, j)
-    {
-      if                        j  < ichildidx {
-        assert result.children[i] == old(node.children[i]);
-        assert result.children[j] == old(node.children[j]);
-        assert old(DisjointSubtrees(node, i, j));
-        assert DisjointSubtrees(result, i, j);
-      } else if                 j == ichildidx {
-        assert result.children[i] == old(node.children[i]);
-        assert old(DisjointSubtrees(node, i, j));
-        assert DisjointSubtrees(result, i, j);
-      } else if i  < ichildidx                 {
-        assert result.children[i] == old(node.children[i]);
-        assert result.children[j] == old(node.children[j]);
-        assert old(DisjointSubtrees(node, i, j));
-        assert DisjointSubtrees(result, i, j);
-      } else if i == ichildidx                 {
-        assert result.children[j] == old(node.children[j]);
-        assert old(DisjointSubtrees(node, i, j));
-        assert DisjointSubtrees(result, i, j);
-      } else                                   {
-        assert result.children[i] == old(node.children[i]);
-        assert result.children[j] == old(node.children[j]);
-        assert old(DisjointSubtrees(node, i, j));
-        assert DisjointSubtrees(result, i, j);
-      }
-    }
+  //   ghost var ichildidx := childidx as int;
+  //   forall i: int, j: int | 0 <= i < j < result.nchildren as int
+  //     ensures DisjointSubtrees(result, i, j)
+  //   {
+  //     if                        j  < ichildidx {
+  //       assert result.children[i] == old(node.children[i]);
+  //       assert result.children[j] == old(node.children[j]);
+  //       assert old(DisjointSubtrees(node, i, j));
+  //       assert DisjointSubtrees(result, i, j);
+  //     } else if                 j == ichildidx {
+  //       assert result.children[i] == old(node.children[i]);
+  //       assert old(DisjointSubtrees(node, i, j));
+  //       assert DisjointSubtrees(result, i, j);
+  //     } else if i  < ichildidx                 {
+  //       assert result.children[i] == old(node.children[i]);
+  //       assert result.children[j] == old(node.children[j]);
+  //       assert old(DisjointSubtrees(node, i, j));
+  //       assert DisjointSubtrees(result, i, j);
+  //     } else if i == ichildidx                 {
+  //       assert result.children[j] == old(node.children[j]);
+  //       assert old(DisjointSubtrees(node, i, j));
+  //       assert DisjointSubtrees(result, i, j);
+  //     } else                                   {
+  //       assert result.children[i] == old(node.children[i]);
+  //       assert result.children[j] == old(node.children[j]);
+  //       assert old(DisjointSubtrees(node, i, j));
+  //       assert DisjointSubtrees(result, i, j);
+  //     }
+  //   }
 
-    forall i | 0 <= i < result.nchildren
-      ensures WFShape(result.children[i])
-    {
-      if i < childidx {
-        assert old(DisjointSubtrees(node, i as int, childidx as int));
-      } else if i == childidx {
-      } else {
-        assert old(DisjointSubtrees(node, childidx as int, i as int));
-      }
-    }
-  }
+  //   forall i | 0 <= i < result.nchildren
+  //     ensures WFShape(result.children[i])
+  //   {
+  //     if i < childidx {
+  //       assert old(DisjointSubtrees(node, i as int, childidx as int));
+  //     } else if i == childidx {
+  //     } else {
+  //       assert old(DisjointSubtrees(node, childidx as int, i as int));
+  //     }
+  //   }
+  // }
 
-  method InsertIndexChildIsNotFull(oldnode: Node, key: Key, value: Value, childidx: uint64) returns (result: Node)
-    requires WFShape(oldnode)
-    requires BSWF(I(oldnode))
-    requires oldnode.Index?
-    requires childidx as int == BSChildFor(I(oldnode), key)
-    requires !Full(oldnode.children[childidx])
-    ensures WFShape(result)
-    ensures result.height == oldnode.height
-    ensures fresh(result.repr - oldnode.repr)
-    ensures BSWF(I(result))
-    ensures BSInterpretation(I(result)) == BSInterpretation(old(I(oldnode)))[key := value]
-    modifies oldnode.children, oldnode.children[childidx].repr
-    decreases oldnode.height, 1
-  {
-    ghost var node := I(oldnode);
-    ghost var pos := childidx as int;
-    reveal_BSWF();
-    assert BSWF(I(oldnode).children[childidx]);
+  // method InsertIndexChildIsNotFull(oldnode: Node, key: Key, value: Value, childidx: uint64) returns (result: Node)
+  //   requires WFShape(oldnode)
+  //   requires BSWF(I(oldnode))
+  //   requires oldnode.Index?
+  //   requires childidx as int == BSChildFor(I(oldnode), key)
+  //   requires !Full(oldnode.children[childidx])
+  //   ensures WFShape(result)
+  //   ensures result.height == oldnode.height
+  //   ensures fresh(result.repr - oldnode.repr)
+  //   ensures BSWF(I(result))
+  //   ensures BSInterpretation(I(result)) == BSInterpretation(old(I(oldnode)))[key := value]
+  //   modifies oldnode.children, oldnode.children[childidx].repr
+  //   decreases oldnode.height, 1
+  // {
+  //   ghost var node := I(oldnode);
+  //   ghost var pos := childidx as int;
+  //   reveal_BSWF();
+  //   assert BSWF(I(oldnode).children[childidx]);
 
-    result := InsertIndexChildIsNotFullHelper(oldnode, key, value, childidx);
+  //   result := InsertIndexChildIsNotFullHelper(oldnode, key, value, childidx);
 
-    ghost var newnode := I(result);
-    ghost var newchild := I(result.children[childidx]);
-    reveal_BSChildFor();
-    reveal_BSInterpretation();
-    forall i | 0 <= i < |newnode.children|
-      ensures newnode.children[i] == node.children[pos := newchild][i]
-    {
-      if i < pos {
-        assert old(DisjointSubtrees(oldnode, i, pos));
-      } else if i == pos {
-      } else {
-        assert old(DisjointSubtrees(oldnode, pos, i));
-      }
-    }
-    reveal_BSAllKeys();
-    BS.RecursiveInsertIsCorrect(node, key, value, pos, newnode, newchild);
-  }
+  //   ghost var newnode := I(result);
+  //   ghost var newchild := I(result.children[childidx]);
+  //   reveal_BSChildFor();
+  //   reveal_BSInterpretation();
+  //   forall i | 0 <= i < |newnode.children|
+  //     ensures newnode.children[i] == node.children[pos := newchild][i]
+  //   {
+  //     if i < pos {
+  //       assert old(DisjointSubtrees(oldnode, i, pos));
+  //     } else if i == pos {
+  //     } else {
+  //       assert old(DisjointSubtrees(oldnode, pos, i));
+  //     }
+  //   }
+  //   reveal_BSAllKeys();
+  //   BS.RecursiveInsertIsCorrect(node, key, value, pos, newnode, newchild);
+  // }
   
-  method InsertIndex(node: Node, key: Key, value: Value) returns (result: Node)
-    requires WFShape(node)
-    requires BSWF(I(node))
-    requires node.Index?
-    requires !Full(node)
-    // ensures WFShape(result)
-    //ensures result.height == node.height
-    // ensures fresh(result.repr - node.repr)
-    //ensures BSWF(I(result))
-    //ensures BSInterpretation(I(result)) == BSInterpretation(old(I(node)))[key := value]
-    //ensures BSAllKeys(I(result)) <= old(BSAllKeys(I(node))) + {key}
-    modifies node.repr
-    decreases node.height, 2
-  {
-    reveal_BSWF();
-    reveal_BSSplitChildOfIndex();
-    reveal_BSChildFor();
+  // method InsertIndex(node: Node, key: Key, value: Value) returns (result: Node)
+  //   requires WFShape(node)
+  //   requires BSWF(I(node))
+  //   requires node.Index?
+  //   requires !Full(node)
+  //   // ensures WFShape(result)
+  //   //ensures result.height == node.height
+  //   // ensures fresh(result.repr - node.repr)
+  //   //ensures BSWF(I(result))
+  //   //ensures BSInterpretation(I(result)) == BSInterpretation(old(I(node)))[key := value]
+  //   //ensures BSAllKeys(I(result)) <= old(BSAllKeys(I(node))) + {key}
+  //   modifies node.repr
+  //   decreases node.height, 2
+  // {
+  //   reveal_BSWF();
+  //   reveal_BSSplitChildOfIndex();
+  //   reveal_BSChildFor();
     
-    var posplus1 := BS.Keys.ArrayLargestLtePlus1(node.pivots, 0, node.nchildren-1, key);
-    if Full(node.children[posplus1]) {
-      ghost var wit;
-      result, wit := SplitChildOfIndex(node, posplus1);
-      BS.SplitChildOfIndexPreservesWF(old(I(node)), I(result), posplus1 as int, wit);
-      if BS.Keys.lte(result.pivots[posplus1], key) {
-        posplus1 := posplus1 + 1;
-        BS.Keys.LargestLteIsUnique2(result.pivots[..result.nchildren-1], key, posplus1 as int - 1);
-      } else {
-        BS.Keys.LargestLteIsUnique2(result.pivots[..result.nchildren-1], key, posplus1 as int - 1);
-      }
-    } else {
-      result := node;
-    }
+  //   var posplus1 := BS.Keys.ArrayLargestLtePlus1(node.pivots, 0, node.nchildren-1, key);
+  //   if Full(node.children[posplus1]) {
+  //     ghost var wit;
+  //     result, wit := SplitChildOfIndex(node, posplus1);
+  //     BS.SplitChildOfIndexPreservesWF(old(I(node)), I(result), posplus1 as int, wit);
+  //     if BS.Keys.lte(result.pivots[posplus1], key) {
+  //       posplus1 := posplus1 + 1;
+  //       BS.Keys.LargestLteIsUnique2(result.pivots[..result.nchildren-1], key, posplus1 as int - 1);
+  //     } else {
+  //       BS.Keys.LargestLteIsUnique2(result.pivots[..result.nchildren-1], key, posplus1 as int - 1);
+  //     }
+  //   } else {
+  //     result := node;
+  //   }
 
-    assert WFShape(result);
-    assert BSWF(I(result));
-    assert result.Index?;
-    assert posplus1 as int == BSChildFor(I(result), key);
-    assert !Full(result.children[posplus1]);
-    result := InsertIndexChildIsNotFull(result, key, value, posplus1);
-  }
+  //   assert WFShape(result);
+  //   assert BSWF(I(result));
+  //   assert result.Index?;
+  //   assert posplus1 as int == BSChildFor(I(result), key);
+  //   assert !Full(result.children[posplus1]);
+  //   result := InsertIndexChildIsNotFull(result, key, value, posplus1);
+  // }
 
-  method InsertNode(node: Node, key: Key, value: Value) returns (result: Node)
-    requires WFShape(node)
-    requires BSWF(I(node))
-    requires !Full(node)
-    ensures WFShape(result)
-    ensures result.height == node.height
-    ensures fresh(result.repr - node.repr)
-    ensures BSWF(I(result))
-    ensures BSInterpretation(I(result)) == BSInterpretation(old(I(node)))[key := value]
-    ensures BSAllKeys(I(result)) <= old(BSAllKeys(I(node))) + {key}
-    modifies node.repr
-    decreases node.height, 3
-  {
-    if node.Leaf? {
-      result := InsertLeaf(node, key, value);
-    } else {
-      result := InsertIndex(node, key, value);
-    }
-  }
+  // method InsertNode(node: Node, key: Key, value: Value) returns (result: Node)
+  //   requires WFShape(node)
+  //   requires BSWF(I(node))
+  //   requires !Full(node)
+  //   ensures WFShape(result)
+  //   ensures result.height == node.height
+  //   ensures fresh(result.repr - node.repr)
+  //   ensures BSWF(I(result))
+  //   ensures BSInterpretation(I(result)) == BSInterpretation(old(I(node)))[key := value]
+  //   ensures BSAllKeys(I(result)) <= old(BSAllKeys(I(node))) + {key}
+  //   modifies node.repr
+  //   decreases node.height, 3
+  // {
+  //   if node.Leaf? {
+  //     result := InsertLeaf(node, key, value);
+  //   } else {
+  //     result := InsertIndex(node, key, value);
+  //   }
+  // }
 }
 
 // module TestBtreeSpec refines BtreeSpec {
